src/Language/PlutusIR/Analysis/Purity.v
@@ -1,0 +1,87 @@
+From Coq Require Import
+  Strings.String
+  Lists.List
+.
+
+From PlutusCert Require Import
+  Language.PlutusIR
+  Semantics.Dynamic.Values
+  Util.List
+  .
+
+Import NamedTerm.
+Import ListNotations.
+
+Open Scope bool_scope.
+
+Inductive binder_info :=
+  | let_bound : Strictness -> binder_info
+  | lambda_bound
+.
+
+Definition ctx := list (string * binder_info).
+
+(* Pure terms include values or variables that are known to be bound to values *)
+Inductive is_pure (Γ : ctx) : Term -> Type :=
+
+  | is_pure_value : forall t,
+      value t ->
+      ~(is_error t) ->
+      is_pure Γ t
+
+  | is_pure_var_let : forall x,
+      Lookup x (let_bound Strict) Γ ->
+      is_pure Γ (Var x)
+
+  | is_pure_var_lambda : forall x,
+      Lookup x lambda_bound Γ ->
+      is_pure Γ (Var x)
+.
+
+Definition is_errorb (t : Term) : bool :=
+  match t with
+    | Error _ => true
+    | _       => false
+  end.
+
+Definition is_pureb (Γ : ctx) (t : Term) : bool :=
+  match t with
+  | Var x =>
+    match lookup x Γ with
+      | Datatypes.Some lambda_bound => true
+      | Datatypes.Some (let_bound Strict) => true
+      | Datatypes.Some (let_bound NonStrict) => false
+      | _ => false
+    end
+  | _     => is_value t && negb (is_errorb t)
+  end
+.
+
+(* An approximation of bindings that are pure, they will not diverge when evaluated *)
+Inductive pure_binding (Γ : ctx) : Binding -> Prop :=
+
+  | pb_term_non_strict : forall vd t,
+      pure_binding Γ (TermBind NonStrict vd t)
+
+  | pb_term_strict_val : forall vd t,
+      is_pure Γ t ->
+      pure_binding Γ (TermBind Strict vd t)
+
+  | pb_data : forall dtd,
+      pure_binding Γ (DatatypeBind dtd)
+
+  | pb_type : forall tvd ty,
+      pure_binding Γ (TypeBind tvd ty)
+.
+
+Definition is_pure_binding (Γ : ctx) (b : Binding) : bool :=
+    match b with
+      | TermBind NonStrict vd t => true
+      | TermBind Strict vd t    => is_value t
+      | DatatypeBind dtd        => true
+      | TypeBind tvd ty         => true
+    end
+.
+
+Lemma is_pure_binding_pure_binding : forall Γ b, is_pure_binding Γ b = true -> pure_binding Γ b.
+Admitted.
