notes/status-transl-rels.md
@@ -1,12 +1,12 @@
 |    TRANSFORMATION    | TRANSLATION RELATION                     |  PRE          | POST        | DECISION PROCEDURE           |  SEMANTIC PRESERVATION |
 |----------------------|------------------------------------------|---------------|-------------|------------------------------|-------------------------
-|Inline                | ✓ inline                                 | unique        |             | bool, option, fuel -> ...    |                        |
-|FloatLet              | … LetMerge is not optional, perhaps fine |               |             | … tactics                    |                        |
-|DeadCode              | ✓ use `well-scoped`                      | unique        |             | Mostly commented out         | … WIP                  |
+|Inline                | ✓ `inline`                               | unique        |             | bool, option, fuel -> ...    |                        |
+|FloatLet              | ✓ `let_float` \*                         |               |             | … tactics                    |                        |
+|DeadCode              | ✓ `dead_code` \*                         | unique        |             | Mostly commented out         | … WIP                  |
 |Rename                | ✓ `rename`                               |               | unique      |                              |                        |
 |ThunkRecursions       | ✓ `thunk_rec`                            |               | _ -> _ type |                              |                        |
 |Beta                  | ✓ `extract_bindings`                     |               |             |                              |                        |
-|RecSplit              | ✓ `split_rec` (todo: use well-scoped)    |               |             |                              |                        |
+|RecSplit              | ✓ `split_rec` \*                         |               |             |                              |                        |
 |Unwrap                | ✓ `unwrap_cancel`                        |               |             |                              |                        |
 |LetTypes              | ✓ `ty_let`                               |               | no let type |                              |                        |
 |Scott Enc             | …                                        |               | no let data | … eq_refl (Term_eqb)         |                        |
@@ -15,3 +15,4 @@
 |LetNonStrict          | ✓ `let_non_strict`                       |               |             |                              |                        |
 
 
+\* : use well-scoped
